@prefix skos: <http://www.w3.org/2004/02/skos/core#> .
@prefix dct:  <http://purl.org/dc/terms/> .
@prefix bgim: <https://grupo5-vespoc.github.io/Board-Game-Interaction-Mechanics/bgim-skos#> .

bgim:BoardGameInteractionScheme
    a skos:ConceptScheme ;
    dct:title "Board Game Interaction Mechanics"@en ;
    dct:description "Controlled vocabulary describing interaction mechanics in board games."@en ;
    skos:prefLabel "Board Game Interaction Mechanics"@en ;
    skos:hasTopConcept bgim:Cooperation , bgim:Competition .

bgim:Cooperation
    a skos:Concept ;
    skos:prefLabel "Cooperation"@en ;
    skos:definition "Interaction mechanic in which players collaborate to achieve a shared objective."@en ;
    skos:topConceptOf bgim:BoardGameInteractionScheme ;
    skos:inScheme bgim:BoardGameInteractionScheme .

bgim:Competition
    a skos:Concept ;
    skos:prefLabel "Competition"@en ;
    skos:definition "Interaction mechanic in which players oppose each other to win the game."@en ;
    skos:topConceptOf bgim:BoardGameInteractionScheme ;
    skos:inScheme bgim:BoardGameInteractionScheme .
